GCR.v
@@ -112,13 +112,13 @@ Qed.
   end : gcr.
 
 Lemma oneinit_or_onecr_from_gcr : forall ad t tid,
-  region_exclusivity t ->
+  term_init_cr_exc t ->
   (* --- *)
   gcr t (R_tid tid) = R_ad ad ->
   (one_init ad t \/ one_cr ad t).
 Proof.
   intros * Hregexc Hgcr. assert (Hregexc' := Hregexc).
-  induction t; kappa; invc_regexc; repeat spec; try solve [invc Hgcr];
+  induction t; kappa; invc_tice; repeat spec; try solve [invc Hgcr];
   destruct (Hregexc ad) as [[? | ?] [[? | ?] _]]; eauto;
   invc_noinit; invc_nocr; eauto with gcr.
 Qed.
@@ -168,11 +168,98 @@ Proof.
 Qed.
 
 (* ------------------------------------------------------------------------- *)
+(* memory regions                                                            *)
+(* ------------------------------------------------------------------------- *)
 
-(* TODO
-Notation "'[[' p1 '..' tc '..' p2 ']]'" := (p2 :: tc ++ p1 :: nil)
-  (at level 40).
-*)
+Theorem mreg_preservation_cstep : forall m1 m2 ths1 ths2 tid e ad,
+  m1 / ths1 ~~[tid, e]~~> m2 / ths2 ->
+  ad < #m1 ->
+  m1[ad].R = m2[ad].R.
+Proof.
+  intros. invc_cstep; trivial. invc_mstep; sigma; trivial; omicron; trivial.
+Qed.
+
+Theorem mreg_preservation_rstep : forall m1 m2 ths1 ths2 tid e ad,
+  m1 / ths1 ~~~[tid, e]~~> m2 / ths2 ->
+  ad < #m1 ->
+  m1[ad].R = m2[ad].R.
+Proof.
+  intros. invc_ostep; eauto using mreg_preservation_cstep.
+  repeat omicron; upsilon; eauto using mreg_preservation_cstep;
+  invc_cstep; invc_mstep; sigma; auto.
+Qed.
+
+Theorem mreg_preservation_ustep : forall m1 m2 ths1 ths2 tc ad,
+  m1 / ths1 ~~[tc]~~>* m2 / ths2 ->
+  ad < #m1 ->
+  m1[ad].R = m2[ad].R.
+Proof.
+  intros. ind_ustep; trivial. rewrite IHmultistep;
+  eauto using ustep_nondecreasing_memory_size, mreg_preservation_rstep.
+Qed.
+
+(* ------------------------------------------------------------------------- *)
+(*                                                                           *)
+(* ------------------------------------------------------------------------- *)
+
+Ltac destruct_invariants :=
+  repeat match goal with
+  | H : invariants _ _       |- _ =>
+    unfold invariants in H; decompose record H; clear H
+  | H : forall_program _ _ _ |- _ =>
+    destruct H
+  end.
+
+Corollary rstep_ptyp_for_write : forall m1 m2 ths1 ths2 tid ad' t',
+  invariants m1 ths1 ->
+  (* --- *)
+  m1 / ths1 ~~~[tid, e_write ad' t']~~> m2 / ths2 ->
+  exists T, m1[ad'].T = `w&T`.
+Proof.
+  intros. destruct_invariants. invc_ostep. invc_cstep. invc_mstep.
+  eauto using  ptyp_for_write. 
+Qed.
+
+Local Lemma same_pointer_type :
+  forall m1 mA mB m2 ths1 thsA thsB ths2 tc tid1 tid2 e1 e2 ad,
+    invariants m1 ths1 ->
+    (* --- *)
+    ad < #m1 ->
+    m1 / ths1 ~~~[tid1, e1]~~>  mA / thsA ->
+    mA / thsA  ~~[tc      ]~~>* mB / thsB ->
+    mB / thsB ~~~[tid2, e2]~~>  m2 / ths2 ->
+    (m1[ad].T = mA[ad].T /\ mA[ad].T = mB[ad].T /\ mB[ad].T = m2[ad].T).
+Proof.
+  intros.
+  assert (ad < #mA) by eauto using rstep_nondecreasing_memory_size.
+  assert (ad < #mB) by eauto using ustep_nondecreasing_memory_size.
+  assert (ad < #m2) by eauto using rstep_nondecreasing_memory_size.
+  assert (HtA : m1[ad].T = mA[ad].T) by eauto using ptyp_preservation_rstep.
+  assert (HtB : mA[ad].T = mB[ad].T) by eauto using ptyp_preservation_ustep.
+  assert (Ht2 : mB[ad].T = m2[ad].T) by eauto using ptyp_preservation_rstep.
+  eauto.
+Qed.
+
+Local Lemma same_regions :
+  forall m1 mA mB m2 ths1 thsA thsB ths2 tc tid1 tid2 e1 e2 ad,
+    invariants m1 ths1 ->
+    (* --- *)
+    ad < #m1 ->
+    m1 / ths1 ~~~[tid1, e1]~~>  mA / thsA ->
+    mA / thsA  ~~[tc      ]~~>* mB / thsB ->
+    mB / thsB ~~~[tid2, e2]~~>  m2 / ths2 ->
+    m1[ad].R = mB[ad].R.
+Proof.
+  intros.
+  assert (ad < #mA) by eauto using rstep_nondecreasing_memory_size.
+  assert (ad < #mB) by eauto using ustep_nondecreasing_memory_size.
+  assert (HrA : m1[ad].R = mA[ad].R) by eauto using mreg_preservation_rstep.
+  assert (HrB : mA[ad].R = mB[ad].R) by eauto using mreg_preservation_ustep.
+  rewrite HrB in HrA.
+  assumption.
+Qed.
+
+(* ------------------------------------------------------------------------- *)
 
 Local Lemma _destruct_ustep2 : forall tc m1 m3 ths1 ths3 tid e,
   m1 / ths1 ~~[tc ++ (tid, e) :: nil]~~>* m3 / ths3 ->
@@ -210,6 +297,55 @@ Ltac destruct_ustep3 :=
       as [mA [thsA [mB [thsB [H1A [HAB HB2]]]]]]
   end.
 
+(* TODO: posso usar consistent_term *)
+Local Lemma uninitialized_from_oneinit : forall m ths tid ad,
+  forall_threads ths (valid_term m) ->
+  unique_initializers m ths ->
+  (* --- *)
+  one_init ad ths[tid] ->
+  m[ad].t = None.
+Proof.
+  intros * ? Hui ?.
+  assert (Had : ad < #m) by eauto using oneinit_ad_bound.
+  destruct (Hui ad Had). opt_dec (m[ad].t); trivial.
+  spec. exfalso. eauto using noinit_oneinit_contradiction.
+Qed.
+
+Local Lemma uninitialized_inheritance_rstep : forall m1 m2 ths1 ths2 tid e ad,
+  m2[ad].t = None ->
+  m1 / ths1 ~~~[tid, e]~~> m2 / ths2 ->
+  m1[ad].t = None.
+Proof.
+  intros. invc_ostep; invc_cstep; try invc_mstep; sigma; upsilon; trivial.
+  repeat omicron; trivial.
+Qed.
+
+Local Lemma uninitialized_inheritance_ustep : forall m1 m2 ths1 ths2 tc ad,
+  m2[ad].t = None ->
+  m1 / ths1 ~~[tc]~~>* m2 / ths2 ->
+  m1[ad].t = None.
+Proof.
+  intros. ind_ustep; eauto using uninitialized_inheritance_rstep. 
+Qed.
+
+Local Lemma todo : forall m1 m2 ths1 ths2 tid1 tid2 tc ad,
+  invariants m1 ths1 ->
+  invariants m2 ths2 ->
+  (* --- *)
+  ad < #m1 ->
+  tid1 <> tid2 ->
+  one_init ad ths1[tid1] ->
+  m1 / ths1 ~~[tc]~~>* m2 / ths2 ->
+  one_init ad ths2[tid2] ->
+  False.
+Proof.
+  intros. ind_ustep; eauto using ui_oneinit_contradiction with inva.
+  assert (invariants m2 ths2) by eauto using invariants_preservation_ustep.
+  repeat spec.
+  (* WIP *)
+  eapply IHmultistep. clear IHmultistep.
+Qed.
+
 Theorem safety_write_read : forall m1 m2 ths1 ths2 tc tc' tid1 tid2 ad t1 t2,
   tid1 <> tid2 ->
   invariants m1 ths1 ->
@@ -222,57 +358,61 @@ Proof.
   assert (invariants mB thsB) by eauto using invariants_preservation_ustep.
   assert (invariants m2 ths2) by eauto using invariants_preservation_rstep.
 
-  assert (exists T, m1[ad].T = `w&T`) as [T ?] by admit.
-  assert (mB[ad].T = `w&T`)                    by admit.
+  assert (ad < #m1) by (repeat (invc_ostep; invc_cstep; invc_mstep); trivial).
 
-  assert (gcr ths1[tid1] (R_tid tid1) = m1[ad].R)
+  assert (exists T, m1[ad].T = `w&T`)
+    as [T Hptyp1]
+    by eauto using rstep_ptyp_for_write.
+  assert (m1[ad].T = mA[ad].T /\ mA[ad].T = mB[ad].T /\ mB[ad].T = m2[ad].T)
+    as [HptypA [HptypB Hptyp2]]
+    by eauto using same_pointer_type.
+  rewrite Hptyp1 in HptypA. symmetry in HptypA.
+  rewrite HptypA in HptypB. symmetry in HptypB.
+  rewrite HptypB in Hptyp2. symmetry in Hptyp2.
+
+  assert (Hgcr1 : gcr ths1[tid1] (R_tid tid1) = m1[ad].R)
     by eauto 7 using rstep_gcr_write with inva.
-  assert (gcr thsB[tid2] (R_tid tid2) = mB[ad].R)
+  assert (HgcrB : gcr thsB[tid2] (R_tid tid2) = mB[ad].R)
     by eauto using rstep_gcr_read with inva.
 
-  assert (HR : m1[ad].R = mB[ad].R) by admit.
+  assert (HR : m1[ad].R = mB[ad].R) by eauto using same_regions.
   rewrite <- HR in *.
 
   destruct (m1[ad].R); eauto using gcr_tid_contradiction with gcr.
+  match goal with H : R_ad ?ad' = _ |- _ => rename ad' into adx end.
 
-  eapply oneinit_or_onecr_from_gcr in H6. 2: admit.
-  eapply oneinit_or_onecr_from_gcr in H7. 2: admit.
-
-Abort.
-
-
+  assert (forall_threads ths1 term_init_cr_exc) by eauto using des_inva_tice.
+  assert (forall_threads thsB term_init_cr_exc) by eauto using des_inva_tice.
+  eapply oneinit_or_onecr_from_gcr in Hgcr1 as [Honeinit1 | Honecr1];
+  eapply oneinit_or_onecr_from_gcr in HgcrB as [HoneinitB | HonecrB];
+  eauto.
+  - assert (one_init adx thsA[tid1]). {
+      repeat (invc_ostep; invc_cstep; invc_mstep). sigma.
+      destruct_invariants. eauto using oneinit_preservation_write.
+    }
+    exfalso. admit.
+  - assert (one_init adx thsA[tid1]). {
+      repeat (invc_ostep; invc_cstep; invc_mstep). sigma.
+      destruct_invariants. eauto using oneinit_preservation_write.
+    }
+    admit.
+  - assert (one_cr adx thsA[tid1]). {
+      repeat (invc_ostep; invc_cstep; invc_mstep). sigma.
+      destruct_invariants. eauto using onecr_preservation_write.
+    }
+    exfalso. admit.
+  - assert (one_cr adx thsA[tid1]). {
+      repeat (invc_ostep; invc_cstep; invc_mstep). sigma.
+      destruct_invariants. eauto using onecr_preservation_write.
+    }
+    admit.
+Qed.
 
 (*
 
-
 ths1, tid1, READ ad   ---- tc1  REL tc2 ACQ tc3 ------->*   ths2, tid2, WRITE ad
 
-m[ad].R = R_ad adx
-
-one_init adx ths1[tid1] \/ one_cr adx ths1[tid1]
-
-one_init adx ths2[tid2] \/ one_cr adx ths2[tid2]
-
-
-init tid1 adx
-init tid2 adx
-
-
-init tid1 adx  X
-cr   tid2 adx
-
-
-cr   tid1 adx
-init tid2 adx
-
-
-cr tid1 adx  X
-cr tid2 adx
-
-
-
 *)
-
 
 Lemma gcr_ad_tid_contradiction : forall tid ad t,
   gcr t (R_ad ad) = R_tid tid ->
