TypeProperties.v
@@ -3,6 +3,6 @@ From Elo Require Export ConsistentTerm.
 From Elo Require Export PointerTypes.
 From Elo Require Export Soundness.
 From Elo Require Export SafeTerm.
-From Elo Require Export ExclusivityInitCR.
+From Elo Require Export Exclusivity.
 From Elo Require Export ConsistentRegions.
 
